Simplifying ValidAddresses

AnyTerm.v
@@ -1,29 +1,36 @@
+From Elo Require Import Util.
 From Elo Require Import Core.
 From Elo Require Import CoreExt.
-From Elo Require Import HasAddress.
 
 (* ------------------------------------------------------------------------- *)
 (* anyt                                                                      *)
 (* ------------------------------------------------------------------------- *)
 
 Inductive anyt (P : tm -> Prop) : tm -> Prop :=
-  | anyt_unit  :                P <{ unit }>     -> anyt P <{ unit }>
-  | anyt_num   : forall n,      P <{ N n }>      -> anyt P <{ N n }>
-  | anyt_ad    : forall ad T,   P <{ &ad :: T }> -> anyt P <{ &ad :: T }>
-  | anyt_new   : forall T t,    anyt P t          -> anyt P <{ new T t }>
-  | anyt_load  : forall t,      anyt P t          -> anyt P <{ *t }>
-  | anyt_asg1  : forall t1 t2,  anyt P t1         -> anyt P <{ t1 = t2 }>
-  | anyt_asg2  : forall t1 t2,  anyt P t2         -> anyt P <{ t1 = t2 }>
-  | anyt_var   : forall x,      P <{ var x }>    -> anyt P <{ var x }>
-  | anyt_fun   : forall x Tx t, anyt P t          -> anyt P <{ fn x Tx --> t }>
-  | anyt_call1 : forall t1 t2,  anyt P t1         -> anyt P <{ call t1 t2 }>
-  | anyt_call2 : forall t1 t2,  anyt P t2         -> anyt P <{ call t1 t2 }>
-  | anyt_seq1  : forall t1 t2,  anyt P t1         -> anyt P <{ t1; t2 }>
-  | anyt_seq2  : forall t1 t2,  anyt P t2         -> anyt P <{ t1; t2 }>
-  | anyt_spawn : forall t,      anyt P t          -> anyt P <{ spawn t }>
+  | anyt_unit   :                P <{ unit }>       -> anyt P <{ unit }>
+  | anyt_num    : forall n,      P <{ N n }>        -> anyt P <{ N n }>
+  | anyt_ad     : forall ad T,   P <{ &ad :: T }>   -> anyt P <{ &ad :: T }>
+  | anyt_new    : forall T t,    P <{ new T t }>    -> anyt P <{ new T t }>
+  | anyt_new1   : forall T t,    anyt P t           -> anyt P <{ new T t }>
+  | anyt_load   : forall t,      P <{ *t }>         -> anyt P <{ *t }>
+  | anyt_load1  : forall t,      anyt P t           -> anyt P <{ *t }>
+  | anyt_asg    : forall t1 t2,  P <{ t1 = t2 }>    -> anyt P <{ t1 = t2 }>
+  | anyt_asg1   : forall t1 t2,  anyt P t1          -> anyt P <{ t1 = t2 }>
+  | anyt_asg2   : forall t1 t2,  anyt P t2          -> anyt P <{ t1 = t2 }>
+  | anyt_var    : forall x,      P <{ var x }>      -> anyt P <{ var x }>
+  | anyt_fun    : forall x Tx t, P <{ fn x Tx t }>  -> anyt P <{ fn x Tx t }>
+  | anyt_fun1   : forall x Tx t, anyt P t           -> anyt P <{ fn x Tx t }>
+  | anyt_call   : forall t1 t2,  P <{ call t1 t2 }> -> anyt P <{ call t1 t2 }>
+  | anyt_call1  : forall t1 t2,  anyt P t1          -> anyt P <{ call t1 t2 }>
+  | anyt_call2  : forall t1 t2,  anyt P t2          -> anyt P <{ call t1 t2 }>
+  | anyt_seq    : forall t1 t2,  P <{ t1; t2 }>     -> anyt P <{ t1; t2 }>
+  | anyt_seq1   : forall t1 t2,  anyt P t1          -> anyt P <{ t1; t2 }>
+  | anyt_seq2   : forall t1 t2,  anyt P t2          -> anyt P <{ t1; t2 }>
+  | anyt_spawn  : forall t,      P <{ spawn t }>    -> anyt P <{ spawn t }>
+  | anyt_spawn1 : forall t,      anyt P t           -> anyt P <{ spawn t }>
   .
 
-(* Generalization, since <v> is inside <t>. *)
+(* Since <v> is inside <t>: *)
 
 Lemma anyt_write_generalization : forall P t t' ad v V,
   anyt P v ->
@@ -41,21 +48,3 @@ Proof.
   intros. induction_step; eauto using anyt.
 Qed.
 
-(* ------------------------------------------------------------------------- *)
-(* has_address                                                               *)
-(* ------------------------------------------------------------------------- *)
-
-Inductive is_address : addr -> tm -> Prop :=
-  | is_ad : forall ad T,
-    is_address ad <{ &ad :: T}>
-  .
-
-Notation "t 'has_address' ad" := (anyt (is_address ad) t)
-  (at level 80, no associativity).
-
-Lemma write_requires_has_address : forall t t' ad v V,
-  t --[EF_Write ad v V]--> t' ->
-  t has_address ad.
-Proof.
-  intros. induction_step; eauto using anyt, is_address.
-Qed.
