ValidAddresses.v
@@ -6,68 +6,126 @@ From Elo Require Import Util.
 From Elo Require Import Array.
 From Elo Require Import Core.
 From Elo Require Import CoreExt.
-From Elo Require Import HasAddress.
+From Elo Require Import AnyTerm.
 
-(* The addresses of a term are valid if they
-are smaller than the length of the memory. *)
+(* ------------------------------------------------------------------------- *)
+(* has_address                                                               *)
+(* ------------------------------------------------------------------------- *)
+
+Inductive is_address : addr -> tm -> Prop :=
+  | is_ad : forall ad T,
+    is_address ad <{ &ad :: T}>
+  .
+
+Notation "t 'has_address' ad" := (anyt (is_address ad) t)
+  (at level 80, no associativity).
+
+Local Lemma write_requires_has_address : forall t t' ad v V,
+  t --[EF_Write ad v V]--> t' ->
+  t has_address ad.
+Proof.
+  intros. induction_step; eauto using anyt, is_address.
+Qed.
+
+Local Ltac inversion_is_address := 
+  match goal with
+  | H : is_address _ _ |- _ => inversion_subst_clear H
+  end.
+
+Local Ltac inversion_has_address := 
+  match goal with
+  | H : _ has_address _ |- _ =>
+      inversion_subst_clear H; try inversion_is_address
+  end.
+
+Local Hint Extern 4 =>
+  try inversion_has_address; try inversion_is_address
+  : has_address_inversion.
+
+(* ------------------------------------------------------------------------- *)
+(* valid-addresses                                                           *)
+(* ------------------------------------------------------------------------- *)
+
+(* The addresses are valid if they are within the bounds of the memory. *)
 Definition valid_addresses (m : mem) (t : tm) :=
-  forall ad, HasAddress ad t -> ad < #m.
+  forall ad, t has_address ad -> ad < #m.
+
+#[export] Hint Unfold valid_addresses : core.
+
+Theorem valid_address_write : forall m t t' ad v V,
+  valid_addresses m t ->
+  t --[EF_Write ad v V]--> t' ->
+  ad < #m.
+Proof. eauto using write_requires_has_address. Qed.
 
 (* ------------------------------------------------------------------------- *)
 (* constructors                                                              *)
 (* ------------------------------------------------------------------------- *)
 
-Local Ltac solve_vad_constructor := 
-  intros; intros ? ?; inversion_ha; eauto.
-
 Local Lemma vad_unit : forall m,
   valid_addresses m <{ unit }>.
-Proof. solve_vad_constructor. Qed.
+Proof. eauto with has_address_inversion. Qed.
+
+Local Lemma vad_num : forall m n,
+  valid_addresses m <{ N n }>.
+Proof. eauto with has_address_inversion. Qed.
 
 Local Lemma vad_new : forall m t T,
   valid_addresses m t ->
   valid_addresses m <{ new T t }>.
-Proof. solve_vad_constructor. Qed.
+Proof. eauto with has_address_inversion. Qed.
 
 Local Lemma vad_load : forall m t,
   valid_addresses m t ->
   valid_addresses m <{ *t }>.
-Proof. solve_vad_constructor. Qed.
+Proof. eauto with has_address_inversion. Qed.
 
 Local Lemma vad_asg : forall m t1 t2,
   valid_addresses m t1 ->
   valid_addresses m t2 ->
   valid_addresses m <{ t1 = t2 }>.
-Proof. solve_vad_constructor. Qed.
+Proof. eauto with has_address_inversion. Qed.
+
+Local Lemma vad_var : forall m x,
+  valid_addresses m <{ var x }>.
+Proof. eauto with has_address_inversion. Qed.
 
 Local Lemma vad_fun : forall m x Tx t,
   valid_addresses m t ->
-  valid_addresses m <{ fn x Tx --> t }>.
-Proof. solve_vad_constructor. Qed.
+  valid_addresses m <{ fn x Tx t }>.
+Proof. eauto with has_address_inversion. Qed.
 
 Local Lemma vad_call : forall m t1 t2,
   valid_addresses m t1 ->
   valid_addresses m t2 ->
   valid_addresses m <{ call t1 t2 }>.
-Proof. solve_vad_constructor. Qed.
+Proof. eauto with has_address_inversion. Qed.
 
 Local Lemma vad_seq : forall m t1 t2,
   valid_addresses m t1 ->
   valid_addresses m t2 ->
   valid_addresses m <{ t1; t2 }>.
-Proof. solve_vad_constructor. Qed.
+Proof. eauto with has_address_inversion. Qed.
 
 Local Lemma vad_spawn : forall m t,
   valid_addresses m t ->
   valid_addresses m <{ spawn t }>.
-Proof. solve_vad_constructor. Qed.
+Proof. eauto with has_address_inversion. Qed.
+
+Local Hint Resolve vad_unit vad_num 
+                   vad_new vad_load vad_asg
+                   vad_var vad_fun vad_call vad_seq vad_spawn
+                   : vad_constructors.
 
 (* ------------------------------------------------------------------------- *)
 (* inversion                                                                 *)
 (* ------------------------------------------------------------------------- *)
 
 Local Ltac solve_vad_inversion := 
-  intros; unfold valid_addresses in *; try split; eauto using HasAddress.
+  intros; try split; eauto using anyt, is_address.
+
+(* vad_unit implicates nothing *)
+(* vad_num implicates nothing *)
 
 Local Lemma inv_vad_ref : forall m ad T,
   valid_addresses m <{ &ad :: T }> ->
@@ -89,8 +147,10 @@ Local Lemma inv_vad_asg : forall m t1 t2,
   valid_addresses m t1 /\ valid_addresses m t2.
 Proof. solve_vad_inversion. Qed.
 
+(* vad_var implicates nothing *)
+
 Local Lemma inv_vad_fun : forall m x Tx t,
-  valid_addresses m <{ fn x Tx --> t }> ->
+  valid_addresses m <{ fn x Tx t }> ->
   valid_addresses m t.
 Proof. solve_vad_inversion. Qed.
 
@@ -110,47 +170,46 @@ Local Lemma inv_vad_spawn : forall m t,
 Proof. solve_vad_inversion. Qed.
 
 Ltac inversion_vad :=
-  match goal with
-  |H: valid_addresses _ <{ & _ :: _ }> |- _ => eapply inv_vad_ref  in H as ?
-  |H: valid_addresses _ <{ new _ _  }> |- _ => eapply inv_vad_new  in H
-  |H: valid_addresses _ <{ * _      }> |- _ => eapply inv_vad_load in H
-  |H: valid_addresses _ <{ _ = _    }> |- _ => eapply inv_vad_asg  in H as [? ?]
-  |H: valid_addresses _ <{ fn _ _ --> _ }> |- _ => eapply inv_vad_fun in H
-  |H: valid_addresses _ <{ call _ _ }> |- _ => eapply inv_vad_call in H as [? ?]
-  |H: valid_addresses _ <{ _ ; _    }> |- _ => eapply inv_vad_seq  in H as [? ?]
-  |H: valid_addresses _ <{ spawn _  }> |- _ => eapply inv_vad_spawn in H
-  end.
+ match goal with
+ | H: valid_addresses _ <{ & _ :: _ }> |- _ => eapply inv_vad_ref  in H as ?
+ | H: valid_addresses _ <{ new _ _  }> |- _ => eapply inv_vad_new  in H
+ | H: valid_addresses _ <{ * _      }> |- _ => eapply inv_vad_load in H
+ | H: valid_addresses _ <{ _ = _    }> |- _ => eapply inv_vad_asg  in H as [? ?]
+ | H: valid_addresses _ <{ fn _ _ _ }> |- _ => eapply inv_vad_fun  in H
+ | H: valid_addresses _ <{ call _ _ }> |- _ => eapply inv_vad_call in H as [? ?]
+ | H: valid_addresses _ <{ _ ; _    }> |- _ => eapply inv_vad_seq  in H as [? ?]
+ | H: valid_addresses _ <{ spawn _  }> |- _ => eapply inv_vad_spawn in H
+ end.
 
 (* ------------------------------------------------------------------------- *)
 (* preservation helpers                                                      *)
 (* ------------------------------------------------------------------------- *)
 
-Local Lemma subst_vad : forall m t tx x,
+Local Lemma mem_add_preserves_vad : forall m t vT,
+  valid_addresses m t ->
+  valid_addresses (m +++ vT) t.
+Proof.
+  intros. intros ? Hha. rewrite add_increments_length.
+  induction Hha; try inversion_vad; eauto with has_address_inversion.
+Qed.
+
+Local Lemma mem_set_preserves_vad : forall m t ad v T,
+  valid_addresses m v ->
+  valid_addresses m t ->
+  valid_addresses m[ad <- (v, T)] t.
+Proof.
+  intros. intros ? Hha. rewrite set_preserves_length.
+  induction Hha; try inversion_vad; eauto with has_address_inversion.
+Qed.
+
+Local Lemma subst_preserves_vad : forall m t tx x,
   valid_addresses m t ->
   valid_addresses m tx ->
   valid_addresses m ([x := tx] t).
 Proof.
-  intros. induction t; try inversion_vad; simpl;
-  eauto using vad_new, vad_load, vad_asg, vad_call, vad_seq, vad_fun, vad_spawn;
-  destruct String.string_dec; subst; trivial;
-  intros ? ?; inversion_ha; unfold valid_addresses in *; eauto.
-Qed.
-
-Local Lemma mem_add_vad : forall m t vTr,
-  valid_addresses m t ->
-  valid_addresses (m +++ vTr) t.
-Proof.
-  intros * ? ? Hha. rewrite add_increments_length.
-  induction Hha; inversion_vad; eauto.
-Qed.
-
-Local Lemma mem_set_vad : forall m t ad v Tr,
-  valid_addresses m v ->
-  valid_addresses m t ->
-  valid_addresses m[ad <- (v, Tr)] t.
-Proof.
-  intros * ? ? ? Hha. rewrite set_preserves_length.
-  induction Hha; inversion_vad; eauto.
+  intros. induction t; try inversion_vad; simpl; eauto with vad_constructors;
+  destruct string_eq_dec; subst; trivial;
+  autounfold in *; eauto with has_address_inversion.
 Qed.
 
 Local Lemma step_spawn_vad_block : forall m t t' block,
@@ -165,24 +224,14 @@ Qed.
 (* term preservation                                                         *)
 (* ------------------------------------------------------------------------- *)
 
-Local Lemma step_none_vad_preservation : forall m t t',
+Local Lemma step_alloc_vad_preservation : forall m t t' v T,
   valid_addresses m t ->
-  t --[EF_None]--> t' ->
-  valid_addresses m t'.
-Proof.
-  intros. induction_step; inversion_vad;  
-  eauto using vad_new, vad_load, vad_asg, vad_fun, vad_call, vad_seq. 
-  inversion_vad. eauto using subst_vad.
-Qed.
-
-Local Lemma step_alloc_vad_preservation : forall m t t' v Tr,
-  valid_addresses m t ->
-  t --[EF_Alloc (#m) v Tr]--> t' ->
-  valid_addresses (m +++ (v, Tr)) t'.
+  t --[EF_Alloc (#m) v T]--> t' ->
+  valid_addresses (m +++ (v, T)) t'.
 Proof.
   intros. induction_step; inversion_vad;
-  eauto using mem_add_vad, vad_new, vad_load, vad_asg, vad_call, vad_seq.
-  intros ? ?. inversion_ha. rewrite add_increments_length. lia.
+  eauto using mem_add_preserves_vad with vad_constructors.
+  intros ? ?. rewrite add_increments_length. inversion_has_address. lia.
 Qed.
 
 Local Lemma step_read_vad_preservation : forall m t t' ad v,
@@ -191,26 +240,31 @@ Local Lemma step_read_vad_preservation : forall m t t' ad v,
   t --[EF_Read ad v]--> t' ->
   valid_addresses m t'.
 Proof.
-  intros. induction_step; inversion_vad;
-  eauto using vad_new, vad_load, vad_asg, vad_call, vad_seq.
+  intros. induction_step; inversion_vad; eauto with vad_constructors.
 Qed.
 
-Local Lemma step_write_vad_preservation : forall m t t' ad v Tr,
+Local Lemma step_write_vad_preservation : forall m t t' ad v T,
   valid_addresses m t ->
-  t --[EF_Write ad v Tr]--> t' ->
-  valid_addresses m[ad <- (v, Tr)] t'.
+  t --[EF_Write ad v T]--> t' ->
+  valid_addresses m[ad <- (v, T)] t'.
 Proof.
-  intros. assert (valid_addresses m v) by shelve.
-  induction_step; inversion_vad;
-  eauto using mem_set_vad, vad_unit, vad_new, vad_load, vad_asg,
-    vad_call, vad_seq.
-  Unshelve. intros ? ?. induction_step; inversion_vad; eauto.
+  intros. assert (valid_addresses m v); induction_step; inversion_vad;
+  eauto using mem_set_preserves_vad with vad_constructors.
 Qed.
 
-Local Corollary mstep_vad_preservation : forall m m' t t' eff,
+Local Lemma step_none_vad_preservation : forall m t t',
+  valid_addresses m t ->
+  t --[EF_None]--> t' ->
+  valid_addresses m t'.
+Proof.
+  intros. induction_step; inversion_vad; eauto with vad_constructors. 
+  inversion_vad. eauto using subst_preserves_vad.
+Qed.
+
+Local Corollary mstep_vad_preservation : forall m m' t t' e,
   forall_memory m (valid_addresses m) ->
   valid_addresses m t ->
-  m / t ==[eff]==> m' / t' ->
+  m / t ==[e]==> m' / t' ->
   valid_addresses m' t'.
 Proof.
   intros. inversion_mstep;
@@ -225,45 +279,43 @@ Local Lemma step_spawn_vad_preservation : forall m t t' block,
   t --[EF_Spawn block]--> t' ->
   valid_addresses m t'.
 Proof.
-  intros. induction_step; inversion_vad;
-  eauto using vad_unit, vad_new, vad_load, vad_asg, vad_call, vad_seq.
+  intros. induction_step; inversion_vad; eauto with vad_constructors.
 Qed.
 
 (* ------------------------------------------------------------------------- *)
 (* memory preservation                                                       *)
 (* ------------------------------------------------------------------------- *)
 
-Local Lemma step_alloc_mem_vad_preservation : forall m t t' v Tr,
+Local Lemma step_alloc_mem_vad_preservation : forall m t t' v T,
   valid_addresses m t ->
   forall_memory m (valid_addresses m) ->
-  t --[EF_Alloc (#m) v Tr]--> t' ->
-  forall_memory  (m +++ (v, Tr)) (valid_addresses (m +++ (v, Tr))).
+  t --[EF_Alloc (#m) v T]--> t' ->
+  forall_memory  (m +++ (v, T)) (valid_addresses (m +++ (v, T))).
 Proof.
   intros. intros ad.
   decompose sum (lt_eq_lt_dec ad (#m)); subst; simpl_array;
-  intros ? ?; rewrite add_increments_length;
-  unfold valid_addresses in *; eauto using step_alloc_hasad, Nat.lt_lt_succ_r.
-  simpl in *. inversion_ha.
+  intros ? ?; rewrite add_increments_length; autounfold in *;
+  eauto using anyt_alloc_generalization, Nat.lt_lt_succ_r
+        with has_address_inversion.
 Qed.
 
-Local Lemma step_write_mem_vad_preservation : forall m t t' ad v Tr,
+Local Lemma step_write_mem_vad_preservation : forall m t t' ad v T,
   valid_addresses m t ->
   forall_memory m (valid_addresses m) ->
-  t --[EF_Write ad v Tr]--> t' ->
-  forall_memory m[ad <- (v, Tr)] (valid_addresses m[ad <- (v, Tr)]).
+  t --[EF_Write ad v T]--> t' ->
+  forall_memory m[ad <- (v, T)] (valid_addresses m[ad <- (v, T)]).
 Proof.
   intros. intros ad'. 
-  assert (ad < #m) by eauto using step_write_hasad1.
+  assert (ad < #m) by eauto using write_requires_has_address.
   destruct (Nat.eq_dec ad ad'); subst; simpl_array;
-  intros ? ?; rewrite set_preserves_length;
-  eauto using step_write_hasad2, Nat.lt_lt_succ_r.
-  unfold valid_addresses in *. eauto.
+  intros ? ?; rewrite set_preserves_length; autounfold in *;
+  eauto using anyt_write_generalization, Nat.lt_lt_succ_r.
 Qed.
 
-Local Corollary mstep_mem_vad_preservation : forall m m' t t' eff,
+Local Corollary mstep_mem_vad_preservation : forall m m' t t' e,
   valid_addresses m t ->
   forall_memory m (valid_addresses m) ->
-  m / t ==[eff]==> m' / t' ->
+  m / t ==[e]==> m' / t' ->
   forall_memory m' (valid_addresses m').
 Proof.
   intros. inversion_mstep; trivial;
@@ -274,24 +326,24 @@ Qed.
 (* preservation                                                              *)
 (* ------------------------------------------------------------------------- *)
 
-Theorem valid_addresses_term_preservation : forall m m' ths ths' tid eff,
+Theorem valid_addresses_term_preservation : forall m m' ths ths' tid e,
   forall_program m ths (valid_addresses m) ->
-  m / ths ~~[tid, eff]~~> m' / ths' ->
+  m / ths ~~[tid, e]~~> m' / ths' ->
   forall_threads ths' (valid_addresses m').
 Proof.
   intros * [? ?]. intros. eapply cstep_preservation; eauto.
   - eauto using mstep_vad_preservation.
-  - intros. intros ? ?. unfold valid_addresses in *. inversion_mstep; eauto;
+  - intros. intros ? ?. autounfold in *. inversion_mstep; eauto;
     (rewrite add_increments_length || rewrite set_preserves_length);
     eauto using Nat.lt_lt_succ_r.
   - eauto using step_spawn_vad_block.
   - eauto using step_spawn_vad_preservation.
-  - unfold thread_default. eauto using vad_unit.
+  - unfold thread_default. eauto with vad_constructors.
 Qed.
 
-Theorem valid_addresses_memory_preservation : forall m m' ths ths' tid eff,
+Theorem valid_addresses_memory_preservation : forall m m' ths ths' tid e,
   forall_program m ths (valid_addresses m) ->
-  m / ths ~~[tid, eff]~~> m' / ths' ->
+  m / ths ~~[tid, e]~~> m' / ths' ->
   forall_memory m' (valid_addresses m').
 Proof.
   intros * [? ?]. intros.
